Fixing deterministic channel, which was broken in recent changes

PolarCodes/deterministic_channelScript.sml
@@ -4,10 +4,12 @@ Ancestors arithmetic bitstring bxor_lemmas degenerate_distribution lifting memor
 
 Libs dep_rewrite realLib liftLib transferLib;
 
+(* It may be convenient to use GSYM degenerate_prob_space_def when working with
+   the appropriate prob space *)
 Definition deterministic_channel0_def:
   deterministic_channel0 (f : α -> β) (S : α -> bool) =
-  (S, λx. degenerate_prob_space (f x) 𝕌(:β))
-  : (α -> bool) # (α -> β m_space)
+  (S, (𝕌(:β), POW (𝕌(:β))), λx. degenerate_distribution (f x))
+  : (α -> bool) # (β algebra) # (α -> β measure)
 End
 
 Theorem wf_memoryless_channel_deterministic_channel0:
@@ -15,16 +17,13 @@ Theorem wf_memoryless_channel_deterministic_channel0:
     wf_memoryless_channel (deterministic_channel0 f S)
 Proof
   rpt gen_tac
-  >> simp[deterministic_channel0_def, wf_memoryless_channel_def]
-  >> conj_tac
-  (* Each output is a probability space *)
-  >- (simp[mcchannel0_def, mcdomain0_def]
-      >> gen_tac >> strip_tac
-      >> simp[degenerate_prob_space_is_prob_space])
-  (* Each output probability space has the same sample space and sigma algebra *)
-  >> rpt gen_tac
-  >> strip_tac
-  >> simp[mcchannel0_def, degenerate_prob_space_def]
+  >> simp[deterministic_channel0_def, wf_memoryless_channel_def,
+          mcdomain0_def, mccodomain0_def, mcchannel0_def, mcsigma0_def,
+          mcevents0_def]
+  >> gen_tac >> strip_tac
+  >> PURE_ONCE_REWRITE_TAC[GSYM degenerate_prob_space_def]
+  >> irule degenerate_prob_space_is_prob_space
+  >> simp[]
 QED
 
 Theorem deterministic_channel0_respects:
